More efficient tactic to close bisimulations using fixpoint witness.

lib/Benchmarks/SmallFilterProof.v
@@ -6,16 +6,17 @@ Notation H := (IncrementalBits.header + BigBits.header).
 Notation A := IncrementalSeparate.aut.
 Notation conf := (P4automaton.configuration (P4A.interp A)).
 
-Definition r_states := (Reachability.reachable_states
-                        IncrementalSeparate.aut
-                        IncrementalBits.Start
-                        BigBits.Parse).
+Definition r_states : {r : Reachability.state_pairs A & Reachability.reachable_states_wit IncrementalBits.Start BigBits.Parse r}.
+  econstructor.
+  unfold Reachability.reachable_states_wit.
+  solve_fp_wit.
+Defined.
 
 Definition top : Relations.rel conf :=
-  fun q1 q2 => List.In (conf_to_state_template q1, conf_to_state_template q2) r_states.
+  fun q1 q2 => List.In (conf_to_state_template q1, conf_to_state_template q2) (projT1 r_states).
 
 Definition top' : Relations.rel (state_template A) :=
-  fun q1 q2 => List.In (q1, q2) r_states.
+  fun q1 q2 => List.In (q1, q2) (projT1 r_states).
 
 
 Declare ML Module "mirrorsolve".
@@ -45,7 +46,7 @@ Lemma prebisim_incremental_sep:
                       cr_rel := btrue;
                    |} q1 q2 ->
   pre_bisimulation A
-                   (wp r_states)
+                   (wp (projT1 r_states))
                    top
                    []
                    (mk_init _ _ _ _ A IncrementalBits.Start BigBits.Parse)
@@ -58,57 +59,6 @@ Proof.
   vm_compute in rel0.
   subst rel0.
 
-  match goal with 
-  | |- pre_bisimulation _ (_ ?rs) _ _ _ _ _ => 
-    set (r_states' := rs);
-    vm_compute in r_states'
-  end.
-  subst r_states'.
-
-  time "build phase" repeat (time "single step" run_bisim top top' r_states).
-
-  eapply PreBisimulationClose;
-  match goal with
-  | H: interp_conf_rel' ?C ?q1 ?q2|- interp_crel _ ?top ?P ?q1 ?q2 =>
-    let H0 := fresh "H0" in
-    assert (H0: interp_entailment' top {| e_prem := P; e_concl := C |}) by (
-      eapply simplify_entailment_correct' with (i := top');
-      eapply compile_simplified_entailment_correct';
-
-      simpl; intros;
-      eapply FirstOrderConfRelSimplified.simplify_eq_zero_fm_corr;
-      eapply CompileFirstOrderConfRelSimplified.compile_simplified_fm_bv_correct;
-
-      crunch_foterm;
-      match goal with
-      | |- ?X => time "smt check pos" check_interp_pos X; admit
-      end
-    );
-    eapply H0;
-    destruct q1, q2;
-    vm_compute in H;
-    repeat match goal with 
-    | H: _ /\ _ |- _ => destruct H
-    end;
-    [
-      (* apply in_checker_conv with (A_eq := fun x y => state_temp_prod_eqdec x y);
-      unfold conf_to_state_template, P4automaton.conf_buf_len, P4automaton.conf_state;
-    
-      repeat match goal with 
-      | H: _ = _ |- _ => erewrite <- H
-      end;
-      exact eq_refl *)
-                    |
-      split; [ vm_compute; (repeat split || assumption) | (intros; exact I)]
-    ] 
-  end.
-  (* Print in_checker_conv. *)
-
-    (* eapply in_checker_conv with (A_eq := fun x y => state_temp_prod_eqdec x y).
-    unfold conf_to_state_template, P4automaton.conf_buf_len, P4automaton.conf_state;
-    
-    repeat match goal with 
-    | H: _ = _ |- _ => erewrite <- H
-    end;
-    exact eq_refl *)
+  time "build phase" repeat (time "single step" run_bisim top top' (projT1 r_states)).
+  time "close phase" close_bisim'' top' r_states.
 Time Admitted.
